\section*{Chapter 6 - Models, Statistical Inference and Learning}

\subsection*{Solution 6.1}

Let $X_1, X_2, ..., X_n \sim \mathrm{Poisson}(\lambda)$.
Estimate $\hat{\lambda} = \frac{1}{n} \sum_{i = 1}^n X_i$.
We have $E(\hat{\lambda}) = \lambda$, so $\mathrm{bias}(\hat{\lambda}) = E(\hat{\lambda}) - \lambda = 0$.
Moreover, $V(\hat{\lambda}) = \frac{\lambda}{n}$, so $\mathrm{se} = \sqrt{\frac{\lambda}{n}}$ and $\mathrm{MSE} = \mathrm{bias}^2 + V(\hat{\lambda}) = \frac{\lambda}{n}$.


\subsection*{Solution 6.2}

Let $X_1, X_2, ..., X_n \sim \mathrm{Uniform}(0, \theta)$.
Let $\hat{\theta} = \mathrm{max}(X_1, X_2, ..., X_n)$.
The cumulative density function is $F(t) = P(\hat{\theta} < t) = \prod P(X_i < t) = t^n$.
So the probability distribution function is $f(t) = F'(t) = nt^{n-1}$.
This gives
\begin{equation*}
    E(\hat{\theta}) = \int_0^{\theta} tf(t) dt = \frac{n}{n+1} \theta, \quad
    \mathrm{bias} = E(\hat{\theta}) - \theta = - \frac{1}{n+1} \theta.
\end{equation*}
So $\hat{\theta}$ is not unbiased ($\frac{n+1}{n} \hat{\theta}$ would be unbiased).
Note that
\begin{equation*}
    \begin{split}
        E(\hat{\theta}^2) &= \int_0^{\theta} t^2 f(t) dt
            = \frac{n}{n+2} \theta^2, \\
        V(\hat{\theta}) &= E(\hat{\theta}^2) - E(\hat{\theta})^2
            = \frac{n}{n+1} \theta^2 - \frac{1}{(n+1)^2} \theta^2
            = \frac{n}{(n+1)^2 (n+2)^2} \theta^2.
    \end{split}
\end{equation*}
We have $\mathrm{se} = \sqrt{V(\hat{\theta})}$.
And the mean squared error is given by
\begin{equation*}
    \mathrm{MSE} = \mathrm{bias}^2 + V(\hat{\theta})
        = \frac{1}{(n+1)^2} \theta^2 + \frac{n}{(n+1)^2 (n+2)} \theta^2
        = \frac{n^2 + 2n + 1}{(n+1)^2 (n+2)} \theta^2
        = \frac{1}{n + 2} \theta^2.
\end{equation*}


\subsection*{Solution 6.3}

Let $X_1, X_2, ..., X_n \sim \mathrm{Uniform}(0, \theta)$.
Let $\hat{\theta} = \frac{2}{n} \sum X_i$.
We have
\begin{equation*}
    E(\hat{\theta}) = \frac{2}{n} \sum_{i=0}^n E(X_i)
        = \theta, \quad
    V(\hat{\theta}) = \frac{2^2}{n^2} \sum_{i = 0}^n V(X_i)
        = \frac{\theta^2}{3n^2}.
\end{equation*}
Therefore, $\mathrm{bias} = 0$, so $\hat{\theta}$ is unbiased, $\mathrm{se} = \frac{\theta}{\sqrt{3}n}$, and $\mathrm{MSE} = \frac{\theta^2}{3n^2}$.
